rename SimulLang into simulirisG

theories/simulation/simulation.v
@@ -6,32 +6,32 @@ From iris.prelude Require Import options.
 Import bi.
 
 (* parameterized over value relation that restricts values passed to functions *)
-Class SimulLang (PROP : bi) (Λ : language) := {
+Class simulirisG (PROP : bi) (Λ : language) := {
   (* state interpretation *)
   state_interp : prog Λ → state Λ → prog Λ → state Λ → PROP;
 }.
 #[global]
-Hint Mode SimulLang + - : typeclass_instances.
+Hint Mode simulirisG + - : typeclass_instances.
 
-Definition progs_are {Λ PROP} `{SimulLang PROP Λ} (P_t P_s : prog Λ) : PROP :=
+Definition progs_are {Λ PROP} `{simulirisG PROP Λ} (P_t P_s : prog Λ) : PROP :=
   (□ ∀ P_t' P_s' σ_t σ_s, state_interp P_t' σ_t P_s' σ_s → ⌜P_t' = P_t⌝ ∧ ⌜P_s' = P_s⌝)%I.
 #[global]
 Hint Mode progs_are - - - + + : typeclass_instances.
 Typeclasses Opaque progs_are.
 
-Global Instance progs_are_persistent {Λ} {PROP} `{s : SimulLang PROP Λ}
+Global Instance progs_are_persistent {Λ} {PROP} `{s : simulirisG PROP Λ}
     (P_s P_t : prog Λ) :
   Persistent (@progs_are Λ PROP s P_s P_t).
 Proof. rewrite /progs_are; apply _. Qed.
 
 (** Typeclass for the simulation relation so we can use the definitions with
    greatest+least fp (stuttering) or just greatest fp (no stuttering). *)
-Class Sim {PROP : bi} {Λ : language} (s : SimulLang PROP Λ) :=
+Class Sim {PROP : bi} {Λ : language} (s : simulirisG PROP Λ) :=
   sim : (val Λ → val Λ → PROP) → (val Λ → val Λ → PROP) → expr Λ → expr Λ → PROP.
 #[global]
 Hint Mode Sim - - - : typeclass_instances.
 
-Class SimE {PROP : bi} {Λ : language} (s : SimulLang PROP Λ) :=
+Class SimE {PROP : bi} {Λ : language} (s : simulirisG PROP Λ) :=
   sim_expr : (val Λ → val Λ → PROP) → (expr Λ → expr Λ → PROP) → expr Λ → expr Λ → PROP.
 #[global]
 Hint Mode SimE - - - : typeclass_instances.
@@ -60,7 +60,7 @@ Section fix_lang.
   Context {PROP : bi} `{!BiBUpd PROP, !BiAffine PROP, !BiPureForall PROP}.
   Context {Λ : language}.
   Context (Ω : val Λ → val Λ → PROP).
-  Context {s : SimulLang PROP Λ}.
+  Context {s : simulirisG PROP Λ}.
 
   Set Default Proof Using "Type*".
 
