theories/simulation/fairness_adequacy.v
@@ -12,7 +12,7 @@ Import bi.
 Section fix_lang.
 Context {PROP : bi} `{!BiBUpd PROP, !BiAffine PROP, !BiPureForall PROP}.
 Context {Λ : language}.
-Context {s : SimulLang PROP Λ}.
+Context {s : simulirisG PROP Λ}.
 
 Set Default Proof Using "Type*".
 
